eve/Src/framework/eiffel2boogie/tests/framing/ownership/observer_one_to_one/f_ooo_observer.e
@@ -59,7 +59,7 @@ invariant
 	subject.observer = Current
 	cache = subject.value
 	subjects = [subject]
-	across subjects as s all s.observers.has (Current) end -- default
+	across subjects as sc all sc.item.observers.has (Current) end -- default
 	owns = [] -- default
 	observers = [] -- default
 
