eve/Src/framework/eiffel2boogie/translation/across/e2b_set_across_handler.e
@@ -1,0 +1,103 @@
+note
+	description: "[
+		TODO
+	]"
+	date: "$Date$"
+	revision: "$Revision$"
+
+class
+	E2B_SET_ACROSS_HANDLER
+
+inherit
+	E2B_ACROSS_HANDLER
+
+create
+	make
+
+feature {NONE} -- Initialization
+
+	make (a_translator: E2B_EXPRESSION_TRANSLATOR; a_loop_expr: LOOP_EXPR_B; a_set_access: ACCESS_B; a_object_test_local: OBJECT_TEST_LOCAL_B)
+			-- Initialize handler.
+		do
+			expression_translator := a_translator
+			loop_expr := a_loop_expr
+			set_access := a_set_access
+			object_test_local := a_object_test_local
+		end
+
+	make_loop (a_loop: LOOP_B; a_object_test_local: OBJECT_TEST_LOCAL_B)
+			-- Initialize handler from loop.
+		do
+			loop_ := a_loop
+			object_test_local := a_object_test_local
+		end
+
+feature -- Access
+
+	loop_: LOOP_B
+	loop_expr: LOOP_EXPR_B
+	set_access: ACCESS_B
+	object_test_local: OBJECT_TEST_LOCAL_B
+
+feature -- Basic operations
+
+	handle_across_expression (a_expr: LOOP_EXPR_B)
+			-- <Precursor>
+		local
+			l_counter: IV_ENTITY
+			l_lower: IV_EXPRESSION
+			l_upper: IV_EXPRESSION
+			l_binop1, l_binop2: IV_BINARY_OPERATION
+			l_and: IV_BINARY_OPERATION
+			l_implies: IV_BINARY_OPERATION
+			l_quantifier: IV_QUANTIFIER
+			l_expression: IV_EXPRESSION
+			l_set: IV_EXPRESSION
+			l_map: IV_MAP_ACCESS
+		do
+				-- Set expression
+			set_access.process (expression_translator)
+			l_set := expression_translator.last_expression
+
+				-- Loop content
+			expression_translator.create_iterator (types.ref)
+			l_counter := expression_translator.last_local
+			expression_translator.locals_map.put (l_counter, object_test_local.position)
+			loop_expr.expression_code.process (expression_translator)
+			l_expression := expression_translator.last_expression
+			expression_translator.locals_map.remove (object_test_local.position)
+
+
+			create l_map.make (l_set, l_counter)
+			create l_implies.make (l_map, "==>", l_expression, types.bool)
+			if loop_expr.is_all then
+				create {IV_FORALL} l_quantifier.make (l_implies)
+			else
+				create {IV_EXISTS} l_quantifier.make (l_implies)
+			end
+			l_quantifier.add_bound_variable (l_counter.name, l_counter.type)
+			expression_translator.set_last_expression (l_quantifier)
+		end
+
+	handle_call_item (a_feature: FEATURE_I)
+			-- <Precursor>
+		do
+			expression_translator.set_last_expression (expression_translator.locals_map.item (object_test_local.position))
+		end
+
+	handle_call_cursor_index (a_feature: FEATURE_I)
+			-- <Precursor>
+		do
+		end
+
+	handle_call_after (a_feature: FEATURE_I)
+			-- <Precursor>
+		do
+		end
+
+	handle_call_forth (a_feature: FEATURE_I)
+			-- <Precursor>
+		do
+		end
+
+end
