eve/Src/framework/eiffel2boogie/translation/e2b_modifies_translator.e
@@ -1,0 +1,13 @@
+note
+	description: "[
+		TODO
+	]"
+	date: "$Date$"
+	revision: "$Revision$"
+
+class
+	E2B_MODIFIES_TRANSLATOR
+
+
+
+end
